calc/recompile.sh
@@ -1,6 +1,6 @@
 #!/bin/bash
 set -xe
-rm *.vo
+rm *.vo || echo "Nothing to clean"
 coqc syntax.v
 coqc types.v
 coqc semantics.v
